Revise the semantics upto the simulation relation

src/opt/Simulation.v
@@ -32,98 +32,107 @@ Section SimulationLocal.
 
   Definition SIM_THREAD :=
     forall (sim_terminal: SIM_TERMINAL)
-      (st1_src:lang_src.(Language.state)) (lc1_src:Local.t) (mem_k_src:Memory.t)
-      (st1_tgt:lang_tgt.(Language.state)) (lc1_tgt:Local.t) (mem_k_tgt:Memory.t), Prop.
+      (st1_src:lang_src.(Language.state)) (lc1_src:Local.t) (sc_k_src:TimeMap.t) (mem_k_src:Memory.t)
+      (st1_tgt:lang_tgt.(Language.state)) (lc1_tgt:Local.t) (sc_k_tgt:TimeMap.t) (mem_k_tgt:Memory.t), Prop.
 
   Definition _sim_thread_step
-             (sim_thread: forall (st1_src:lang_src.(Language.state)) (lc1_src:Local.t) (mem_k_src:Memory.t)
-                            (st1_tgt:lang_tgt.(Language.state)) (lc1_tgt:Local.t) (mem_k_tgt:Memory.t), Prop)
-             st1_src lc1_src mem1_src
-             st1_tgt lc1_tgt mem1_tgt
+             (sim_thread: forall (st1_src:lang_src.(Language.state)) (lc1_src:Local.t) (sc_k_src:TimeMap.t) (mem_k_src:Memory.t)
+                            (st1_tgt:lang_tgt.(Language.state)) (lc1_tgt:Local.t) (sc_k_tgt:TimeMap.t) (mem_k_tgt:Memory.t), Prop)
+             st1_src lc1_src sc1_src mem1_src
+             st1_tgt lc1_tgt sc1_tgt mem1_tgt
     :=
-    forall e_tgt st3_tgt lc3_tgt mem3_tgt
+    forall e_tgt st3_tgt lc3_tgt sc3_tgt mem3_tgt
       (STEP_TGT: Thread.step e_tgt
-                             (Thread.mk _ st1_tgt lc1_tgt mem1_tgt)
-                             (Thread.mk _ st3_tgt lc3_tgt mem3_tgt)),
-    exists e_src st2_src lc2_src mem2_src st3_src lc3_src mem3_src,
+                             (Thread.mk _ st1_tgt lc1_tgt sc1_tgt mem1_tgt)
+                             (Thread.mk _ st3_tgt lc3_tgt sc3_tgt mem3_tgt)),
+    exists e_src st2_src lc2_src sc2_src mem2_src st3_src lc3_src sc3_src mem3_src,
       <<STEPS: rtc (@Thread.tau_step _)
-                   (Thread.mk _ st1_src lc1_src mem1_src)
-                   (Thread.mk _ st2_src lc2_src mem2_src)>> /\
+                   (Thread.mk _ st1_src lc1_src sc1_src mem1_src)
+                   (Thread.mk _ st2_src lc2_src sc2_src mem2_src)>> /\
       <<STEP_SRC: Thread.step e_src
-                              (Thread.mk _ st2_src lc2_src mem2_src)
-                              (Thread.mk _ st3_src lc3_src mem3_src)>> /\
+                              (Thread.mk _ st2_src lc2_src sc2_src mem2_src)
+                              (Thread.mk _ st3_src lc3_src sc3_src mem3_src)>> /\
       <<EVENT: ThreadEvent.get_event e_src = ThreadEvent.get_event e_tgt>> /\
       <<MEMORY2: Memory.sim mem3_tgt mem3_src>> /\
-      <<SIM: sim_thread st3_src lc3_src mem3_src st3_tgt lc3_tgt mem3_tgt>>.
+      <<SIM: sim_thread st3_src lc3_src sc3_src mem3_src st3_tgt lc3_tgt sc3_tgt mem3_tgt>>.
 
   (* TODO: inftau & liveness *)
   Definition _sim_thread
              (sim_thread: SIM_THREAD)
              (sim_terminal: SIM_TERMINAL)
-             (st1_src:lang_src.(Language.state)) (lc1_src:Local.t) (mem_k_src:Memory.t)
-             (st1_tgt:lang_tgt.(Language.state)) (lc1_tgt:Local.t) (mem_k_tgt:Memory.t): Prop :=
-    forall mem1_src mem1_tgt
+             (st1_src:lang_src.(Language.state)) (lc1_src:Local.t) (sc_k_src:TimeMap.t) (mem_k_src:Memory.t)
+             (st1_tgt:lang_tgt.(Language.state)) (lc1_tgt:Local.t) (sc_k_tgt:TimeMap.t) (mem_k_tgt:Memory.t): Prop :=
+    forall sc1_src mem1_src
+      sc1_tgt mem1_tgt
       (MEMORY: Memory.sim mem1_tgt mem1_src)
-      (FUTURE_SRC: Memory.future mem_k_src mem1_src)
-      (FUTURE_TGT: Memory.future mem_k_tgt mem1_tgt)
+      (SC_FUTURE_SRC: TimeMap.le sc_k_src sc1_src)
+      (SC_FUTURE_TGT: TimeMap.le sc_k_tgt sc1_tgt)
+      (MEM_FUTURE_SRC: Memory.future mem_k_src mem1_src)
+      (MEM_FUTURE_TGT: Memory.future mem_k_tgt mem1_tgt)
       (WF_SRC: Local.wf lc1_src mem1_src)
       (WF_TGT: Local.wf lc1_tgt mem1_tgt)
+      (SC_SRC: Memory.closed_timemap sc1_src mem1_src)
+      (SC_TGT: Memory.closed_timemap sc1_tgt mem1_tgt)
       (MEM_SRC: Memory.closed mem1_src)
       (MEM_TGT: Memory.closed mem1_tgt),
       <<TERMINAL:
         forall (TERMINAL_TGT: lang_tgt.(Language.is_terminal) st1_tgt),
-        exists st2_src lc2_src mem2_src,
+        exists st2_src lc2_src sc2_src mem2_src,
           <<STEPS: rtc (@Thread.tau_step _)
-                       (Thread.mk _ st1_src lc1_src mem1_src)
-                       (Thread.mk _ st2_src lc2_src mem2_src)>> /\
+                       (Thread.mk _ st1_src lc1_src sc1_src mem1_src)
+                       (Thread.mk _ st2_src lc2_src sc2_src mem2_src)>> /\
           <<MEMORY: Memory.sim mem1_tgt mem2_src>> /\
           <<TERMINAL_SRC: lang_src.(Language.is_terminal) st2_src>> /\
           <<LOCAL: sim_local lc2_src lc1_tgt>> /\
           <<TERMINAL: sim_terminal st2_src st1_tgt>>>> /\
       <<FUTURE:
-        forall mem2_src
-          (FUTURE_SRC: Memory.future mem1_src mem2_src)
+        forall sc2_src mem2_src
+          (SC_FUTURE_SRC: TimeMap.le sc1_src sc2_src)
+          (MEM_FUTURE_SRC: Memory.future mem1_src mem2_src)
           (WF_SRC: Local.wf lc1_src mem2_src)
+          (SC_SRC: Memory.closed_timemap sc2_src mem2_src)
           (MEM_SRC: Memory.closed mem2_src),
-        exists mem2_tgt,
+        exists sc2_tgt mem2_tgt,
           <<MEMORY: Memory.sim mem2_tgt mem2_src>> /\
-          <<FUTURE_TGT: Memory.future mem1_tgt mem2_tgt>> /\
+          <<SC_FUTURE_TGT: TimeMap.le sc1_tgt sc2_tgt>> /\
+          <<MEM_FUTURE_TGT: Memory.future mem1_tgt mem2_tgt>> /\
           <<WF_TGT: Local.wf lc1_tgt mem2_tgt>> /\
+          <<SC_TGT: Memory.closed_timemap sc2_tgt mem2_tgt>> /\
           <<MEM_TGT: Memory.closed mem2_tgt>>>> /\
       <<PROMISES:
         forall (PROMISES_TGT: lc1_tgt.(Local.promises) = Memory.bot),
-        exists st2_src lc2_src mem2_src,
+        exists st2_src lc2_src sc2_src mem2_src,
           <<STEPS: rtc (@Thread.tau_step _)
-                       (Thread.mk _ st1_src lc1_src mem1_src)
-                       (Thread.mk _ st2_src lc2_src mem2_src)>> /\
+                       (Thread.mk _ st1_src lc1_src sc1_src mem1_src)
+                       (Thread.mk _ st2_src lc2_src sc2_src mem2_src)>> /\
           <<PROMISES_SRC: lc2_src.(Local.promises) = Memory.bot>>>> /\
       <<STEP: _sim_thread_step (sim_thread sim_terminal)
-                               st1_src lc1_src mem1_src
-                               st1_tgt lc1_tgt mem1_tgt>>.
+                               st1_src lc1_src sc1_src mem1_src
+                               st1_tgt lc1_tgt sc1_tgt mem1_tgt>>.
 
-  Lemma _sim_thread_mon: monotone7 _sim_thread.
+  Lemma _sim_thread_mon: monotone9 _sim_thread.
   Proof.
     ii. exploit IN; eauto. i. des.
     splits; eauto. ii.
     exploit STEP; eauto. i. des.
-    eexists _, _, _, _, _, _, _. splits; eauto.
+    eexists _, _, _, _, _, _, _, _, _. splits; eauto.
   Qed.
   Hint Resolve _sim_thread_mon: paco.
 
-  Definition sim_thread: SIM_THREAD := paco7 _sim_thread bot7.
+  Definition sim_thread: SIM_THREAD := paco9 _sim_thread bot9.
 
   Lemma sim_thread_mon
         sim_terminal1 sim_terminal2
         (SIM: sim_terminal1 <2= sim_terminal2):
-    sim_thread sim_terminal1 <6= sim_thread sim_terminal2.
+    sim_thread sim_terminal1 <8= sim_thread sim_terminal2.
   Proof.
     pcofix CIH. i. punfold PR. pfold. ii.
     exploit PR; eauto. i. des.
     splits; auto.
     - i. exploit TERMINAL; eauto. i. des.
-      eexists _, _, _. splits; eauto.
+      eexists _, _, _, _. splits; eauto.
     - ii. exploit STEP; eauto. i. des; [|done].
-      eexists _, _, _, _, _, _, _. splits; eauto.
+      eexists _, _, _, _, _, _, _, _, _. splits; eauto.
   Qed.
 End SimulationLocal.
 Hint Resolve _sim_thread_mon: paco.
@@ -131,47 +140,50 @@ Hint Resolve _sim_thread_mon: paco.
 
 Section Simulation.
   Definition SIM :=
-    forall (ths1_src:Threads.t) (mem_k_src:Memory.t)
-      (ths1_tgt:Threads.t) (mem_k_tgt:Memory.t), Prop.
+    forall (ths1_src:Threads.t) (sc_k_src:TimeMap.t) (mem_k_src:Memory.t)
+      (ths1_tgt:Threads.t) (sc_k_tgt:TimeMap.t) (mem_k_tgt:Memory.t), Prop.
 
   (* TODO: inftau & liveness *)
   Definition _sim
              (sim: SIM)
-             (ths1_src:Threads.t) (mem_k_src:Memory.t)
-             (ths1_tgt:Threads.t) (mem_k_tgt:Memory.t): Prop :=
-    forall mem1_src mem1_tgt
+             (ths1_src:Threads.t) (sc_k_src:TimeMap.t) (mem_k_src:Memory.t)
+             (ths1_tgt:Threads.t) (sc_k_tgt:TimeMap.t) (mem_k_tgt:Memory.t): Prop :=
+    forall sc1_src mem1_src
+      sc1_tgt mem1_tgt
       (MEMORY1: Memory.sim mem1_tgt mem1_src)
-      (WF_SRC: Configuration.wf (Configuration.mk ths1_src mem1_src))
-      (WF_TGT: Configuration.wf (Configuration.mk ths1_tgt mem1_tgt))
-      (CONSISTENT_SRC: Configuration.consistent (Configuration.mk ths1_src mem1_src))
-      (CONSISTENT_TGT: Configuration.consistent (Configuration.mk ths1_tgt mem1_tgt))
-      (FUTURE_SRC: Memory.future mem_k_src mem1_src)
-      (FUTURE_TGT: Memory.future mem_k_tgt mem1_tgt),
+      (WF_SRC: Configuration.wf (Configuration.mk ths1_src sc1_src mem1_src))
+      (WF_TGT: Configuration.wf (Configuration.mk ths1_tgt sc1_tgt mem1_tgt))
+      (CONSISTENT_SRC: Configuration.consistent (Configuration.mk ths1_src sc1_src mem1_src))
+      (CONSISTENT_TGT: Configuration.consistent (Configuration.mk ths1_tgt sc1_tgt mem1_tgt))
+      (SC_FUTURE_SRC: TimeMap.le sc_k_src sc1_src)
+      (SC_FUTURE_TGT: TimeMap.le sc_k_tgt sc1_tgt)
+      (MEM_FUTURE_SRC: Memory.future mem_k_src mem1_src)
+      (MEM_FUTURE_TGT: Memory.future mem_k_tgt mem1_tgt),
       <<TERMINAL:
         forall (TERMINAL_TGT: Threads.is_terminal ths1_tgt),
-        exists ths2_src mem2_src,
-          <<STEPS: rtc Configuration.tau_step (Configuration.mk ths1_src mem1_src) (Configuration.mk ths2_src mem2_src)>> /\
+        exists ths2_src sc2_src mem2_src,
+          <<STEPS: rtc Configuration.tau_step (Configuration.mk ths1_src sc1_src mem1_src) (Configuration.mk ths2_src sc2_src mem2_src)>> /\
           <<MEMORY: Memory.sim mem1_tgt mem2_src>> /\
           <<TERMINAL_SRC: Threads.is_terminal ths2_src>>>> /\
       <<STEP:
-        forall e tid_tgt ths3_tgt mem3_tgt
-          (STEP_TGT: Configuration.step e tid_tgt (Configuration.mk ths1_tgt mem1_tgt) (Configuration.mk ths3_tgt mem3_tgt)),
-        exists e tid_src ths2_src mem2_src ths3_src mem3_src,
-          <<STEPS: rtc Configuration.tau_step (Configuration.mk ths1_src mem1_src) (Configuration.mk ths2_src mem2_src)>> /\
-          <<STEP_SRC: Configuration.step e tid_src (Configuration.mk ths2_src mem2_src) (Configuration.mk ths3_src mem3_src)>> /\
+        forall e tid_tgt ths3_tgt sc3_tgt mem3_tgt
+          (STEP_TGT: Configuration.step e tid_tgt (Configuration.mk ths1_tgt sc1_tgt mem1_tgt) (Configuration.mk ths3_tgt sc3_tgt mem3_tgt)),
+        exists e tid_src ths2_src sc2_src mem2_src ths3_src sc3_src mem3_src,
+          <<STEPS: rtc Configuration.tau_step (Configuration.mk ths1_src sc1_src mem1_src) (Configuration.mk ths2_src sc2_src mem2_src)>> /\
+          <<STEP_SRC: Configuration.step e tid_src (Configuration.mk ths2_src sc2_src mem2_src) (Configuration.mk ths3_src sc3_src mem3_src)>> /\
           <<MEMORY2: Memory.sim mem3_tgt mem3_src>> /\
-          <<SIM: sim ths3_src mem3_src ths3_tgt mem3_tgt>>>>.
+          <<SIM: sim ths3_src sc3_src mem3_src ths3_tgt sc3_tgt mem3_tgt>>>>.
 
-  Lemma _sim_mon: monotone4 _sim.
+  Lemma _sim_mon: monotone6 _sim.
   Proof.
     ii. exploit IN; eauto. i. des.
     splits; eauto. i.
     exploit STEP; eauto. i. des.
-    eexists _, _, _, _, _, _. splits; eauto.
+    eexists _, _, _, _, _, _, _, _. splits; eauto.
   Qed.
   Hint Resolve _sim_mon: paco.
 
-  Definition sim: SIM := paco4 _sim bot4.
+  Definition sim: SIM := paco6 _sim bot6.
 End Simulation.
 Hint Resolve _sim_mon: paco.
 
@@ -179,45 +191,42 @@ Hint Resolve _sim_mon: paco.
 Lemma sim_thread_future
       lang_src lang_tgt
       sim_terminal
-      st_src lc_src mem_k1_src mem_k2_src
-      st_tgt lc_tgt mem_k1_tgt mem_k2_tgt
-      (SIM: @sim_thread lang_src lang_tgt sim_terminal st_src lc_src mem_k1_src st_tgt lc_tgt mem_k1_tgt)
-      (FUTURE_SRC: Memory.future mem_k1_src mem_k2_src)
-      (FUTURE_TGT: Memory.future mem_k1_tgt mem_k2_tgt)
-      (WF_SRC: Local.wf lc_src mem_k2_src)
-      (WF_TGT: Local.wf lc_tgt mem_k2_tgt)
-      (MEM_SRC: Memory.closed mem_k2_src)
-      (MEM_TGT: Memory.closed mem_k2_tgt):
-  sim_thread sim_terminal st_src lc_src mem_k2_src st_tgt lc_tgt mem_k2_tgt.
+      st_src lc_src sc_k1_src sc_k2_src mem_k1_src mem_k2_src
+      st_tgt lc_tgt sc_k1_tgt sc_k2_tgt mem_k1_tgt mem_k2_tgt
+      (SIM: @sim_thread lang_src lang_tgt sim_terminal st_src lc_src sc_k1_src mem_k1_src st_tgt lc_tgt sc_k1_tgt mem_k1_tgt)
+      (SC_FUTURE_SRC: TimeMap.le sc_k1_src sc_k2_src)
+      (SC_FUTURE_TGT: TimeMap.le sc_k1_tgt sc_k2_tgt)
+      (MEM_FUTURE_SRC: Memory.future mem_k1_src mem_k2_src)
+      (MEM_FUTURE_TGT: Memory.future mem_k1_tgt mem_k2_tgt):
+  sim_thread sim_terminal st_src lc_src sc_k2_src mem_k2_src st_tgt lc_tgt sc_k2_tgt mem_k2_tgt.
 Proof.
   pfold. ii.
-  punfold SIM. exploit SIM; eauto.
-  - etrans; eauto.
-  - etrans; eauto.
+  punfold SIM. exploit SIM; (try by etrans; eauto); eauto.
 Qed.
 
 
 Lemma sim_future
-      ths_src mem_k1_src mem_k2_src
-      ths_tgt mem_k1_tgt mem_k2_tgt
-      (SIM: sim ths_src mem_k1_src ths_tgt mem_k1_tgt)
-      (FUTURE_SRC: Memory.future mem_k1_src mem_k2_src)
-      (FUTURE_TGT: Memory.future mem_k1_tgt mem_k2_tgt):
-  sim ths_src mem_k2_src ths_tgt mem_k2_tgt.
+      ths_src sc_k1_src sc_k2_src mem_k1_src mem_k2_src
+      ths_tgt sc_k1_tgt sc_k2_tgt mem_k1_tgt mem_k2_tgt
+      (SIM: sim ths_src sc_k1_src mem_k1_src ths_tgt sc_k1_tgt mem_k1_tgt)
+      (SC_FUTURE_SRC: TimeMap.le sc_k1_src sc_k2_src)
+      (SC_FUTURE_TGT: TimeMap.le sc_k1_tgt sc_k2_tgt)
+      (MEM_FUTURE_SRC: Memory.future mem_k1_src mem_k2_src)
+      (MEM_FUTURE_TGT: Memory.future mem_k1_tgt mem_k2_tgt):
+  sim ths_src sc_k2_src mem_k2_src ths_tgt sc_k2_tgt mem_k2_tgt.
 Proof.
   pfold. ii.
-  punfold SIM. exploit SIM; eauto.
-  - etrans; eauto.
-  - etrans; eauto.
+  punfold SIM. exploit SIM; (try by etrans; eauto); eauto.
 Qed.
 
 Lemma singleton_consistent
-      tid lang st lc mem
+      tid lang st lc sc mem
       (WF: Local.wf lc mem)
+      (SC: Memory.closed_timemap sc mem)
       (MEM: Memory.closed mem)
-      (CONSISTENT: Thread.consistent (Thread.mk lang st lc mem)):
-  <<WF: Configuration.wf (Configuration.mk (IdentMap.singleton tid (existT _ _ st, lc)) mem)>> /\
-  <<CONSISTENT: Configuration.consistent (Configuration.mk (IdentMap.singleton tid (existT _ _ st, lc)) mem)>>.
+      (CONSISTENT: Thread.consistent (Thread.mk lang st lc sc mem)):
+  <<WF: Configuration.wf (Configuration.mk (IdentMap.singleton tid (existT _ _ st, lc)) sc mem)>> /\
+  <<CONSISTENT: Configuration.consistent (Configuration.mk (IdentMap.singleton tid (existT _ _ st, lc)) sc mem)>>.
 Proof.
   econs; ss.
   - econs; ss. econs.
@@ -233,12 +242,13 @@ Proof.
 Qed.
 
 Lemma singleton_consistent_inv
-      tid lang st lc mem
-      (WF: Configuration.wf (Configuration.mk (IdentMap.singleton tid (existT _ _ st, lc)) mem))
-      (CONSISTENT: Configuration.consistent (Configuration.mk (IdentMap.singleton tid (existT _ _ st, lc)) mem)):
+      tid lang st lc sc mem
+      (WF: Configuration.wf (Configuration.mk (IdentMap.singleton tid (existT _ _ st, lc)) sc mem))
+      (CONSISTENT: Configuration.consistent (Configuration.mk (IdentMap.singleton tid (existT _ _ st, lc)) sc mem)):
   <<WF: Local.wf lc mem>> /\
+  <<SC: Memory.closed_timemap sc mem>> /\
   <<MEM: Memory.closed mem>> /\
-  <<CONSISTENT: Thread.consistent (Thread.mk lang st lc mem)>>.
+  <<CONSISTENT: Thread.consistent (Thread.mk lang st lc sc mem)>>.
 Proof.
   inv WF. inv WF0. exploit THREADS; eauto.
   { apply IdentMap.singleton_eq. }
@@ -262,88 +272,99 @@ Lemma sim_step
       lang_src lang_tgt
       sim_terminal
       e_tgt
-      st1_src lc1_src mem1_src
-      st1_tgt lc1_tgt mem1_tgt
-      st3_tgt lc3_tgt mem3_tgt
+      st1_src lc1_src sc1_src mem1_src
+      st1_tgt lc1_tgt sc1_tgt mem1_tgt
+      st3_tgt lc3_tgt sc3_tgt mem3_tgt
       (STEP: @Thread.step lang_tgt e_tgt
-                          (Thread.mk _ st1_tgt lc1_tgt mem1_tgt)
-                          (Thread.mk _ st3_tgt lc3_tgt mem3_tgt))
+                          (Thread.mk _ st1_tgt lc1_tgt sc1_tgt mem1_tgt)
+                          (Thread.mk _ st3_tgt lc3_tgt sc3_tgt mem3_tgt))
       (MEMORY: Memory.sim mem1_tgt mem1_src)
       (WF_SRC: Local.wf lc1_src mem1_src)
       (WF_TGT: Local.wf lc1_tgt mem1_tgt)
+      (SC_SRC: Memory.closed_timemap sc1_src mem1_src)
+      (SC_TGT: Memory.closed_timemap sc1_tgt mem1_tgt)
       (MEM_SRC: Memory.closed mem1_src)
       (MEM_TGT: Memory.closed mem1_tgt)
-      (SIM: sim_thread sim_terminal st1_src lc1_src mem1_src st1_tgt lc1_tgt mem1_tgt):
-  exists e_src st2_src lc2_src mem2_src st3_src lc3_src mem3_src,
+      (SIM: sim_thread sim_terminal st1_src lc1_src sc1_src mem1_src st1_tgt lc1_tgt sc1_tgt mem1_tgt):
+  exists e_src st2_src lc2_src sc2_src mem2_src st3_src lc3_src sc3_src mem3_src,
     <<STEPS: rtc (@Thread.tau_step lang_src)
-                 (Thread.mk _ st1_src lc1_src mem1_src)
-                 (Thread.mk _ st2_src lc2_src mem2_src)>> /\
+                 (Thread.mk _ st1_src lc1_src sc1_src mem1_src)
+                 (Thread.mk _ st2_src lc2_src sc2_src mem2_src)>> /\
     <<STEP: Thread.step e_src
-                        (Thread.mk _ st2_src lc2_src mem2_src)
-                        (Thread.mk _ st3_src lc3_src mem3_src)>> /\
+                        (Thread.mk _ st2_src lc2_src sc2_src mem2_src)
+                        (Thread.mk _ st3_src lc3_src sc3_src mem3_src)>> /\
     <<EVENT: ThreadEvent.get_event e_src = ThreadEvent.get_event e_tgt>> /\
     <<MEMORY: Memory.sim mem3_tgt mem3_src>> /\
     <<WF_SRC: Local.wf lc3_src mem3_src>> /\
     <<WF_TGT: Local.wf lc3_tgt mem3_tgt>> /\
+    <<SC_SRC: Memory.closed_timemap sc3_src mem3_src>> /\
+    <<SC_TGT: Memory.closed_timemap sc3_tgt mem3_tgt>> /\
     <<MEM_SRC: Memory.closed mem3_src>> /\
     <<MEM_TGT: Memory.closed mem3_tgt>> /\
-    <<SIM: sim_thread sim_terminal st3_src lc3_src mem3_src st3_tgt lc3_tgt mem3_tgt>>.
+    <<SIM: sim_thread sim_terminal st3_src lc3_src sc3_src mem3_src st3_tgt lc3_tgt sc3_tgt mem3_tgt>>.
 Proof.
-  exploit Thread.step_future; eauto. s. i. des.
   punfold SIM. exploit SIM; eauto; try refl. i. des.
+  exploit Thread.step_future; eauto. s. i. des.
   exploit STEP0; eauto. i. des; [|done].
   exploit Thread.rtc_step_future; eauto. s. i. des.
   exploit Thread.step_future; eauto. s. i. des.
-  eexists _, _, _, _, _, _, _. splits; eauto.
+  eexists _, _, _, _, _, _, _, _, _. splits; eauto.
 Qed.
 
 Lemma sim_rtc_step
       lang_src lang_tgt
       sim_terminal
-      st1_src lc1_src mem1_src
+      st1_src lc1_src sc1_src mem1_src
       e1_tgt e2_tgt
       (STEPS: rtc (@Thread.tau_step lang_tgt) e1_tgt e2_tgt)
       (MEMORY: Memory.sim e1_tgt.(Thread.memory) mem1_src)
       (WF_SRC: Local.wf lc1_src mem1_src)
       (WF_TGT: Local.wf e1_tgt.(Thread.local) e1_tgt.(Thread.memory))
+      (SC_SRC: Memory.closed_timemap sc1_src mem1_src)
+      (SC_TGT: Memory.closed_timemap e1_tgt.(Thread.sc) e1_tgt.(Thread.memory))
       (MEM_SRC: Memory.closed mem1_src)
       (MEM_TGT: Memory.closed e1_tgt.(Thread.memory))
-      (SIM: sim_thread sim_terminal st1_src lc1_src mem1_src e1_tgt.(Thread.state) e1_tgt.(Thread.local) e1_tgt.(Thread.memory)):
-  exists st2_src lc2_src mem2_src,
+      (SIM: sim_thread sim_terminal st1_src lc1_src sc1_src mem1_src e1_tgt.(Thread.state) e1_tgt.(Thread.local) e1_tgt.(Thread.sc) e1_tgt.(Thread.memory)):
+  exists st2_src lc2_src sc2_src mem2_src,
     <<STEPS: rtc (@Thread.tau_step lang_src)
-                 (Thread.mk _ st1_src lc1_src mem1_src)
-                 (Thread.mk _ st2_src lc2_src mem2_src)>> /\
+                 (Thread.mk _ st1_src lc1_src sc1_src mem1_src)
+                 (Thread.mk _ st2_src lc2_src sc2_src mem2_src)>> /\
     <<MEMORY: Memory.sim e2_tgt.(Thread.memory) mem2_src>> /\
     <<WF_SRC: Local.wf lc2_src mem2_src>> /\
     <<WF_TGT: Local.wf e2_tgt.(Thread.local) e2_tgt.(Thread.memory)>> /\
+    <<SC_SRC: Memory.closed_timemap sc2_src mem2_src>> /\
+    <<SC_TGT: Memory.closed_timemap e2_tgt.(Thread.sc) e2_tgt.(Thread.memory)>> /\
     <<MEM_SRC: Memory.closed mem2_src>> /\
     <<MEM_TGT: Memory.closed e2_tgt.(Thread.memory)>> /\
-    <<SIM: sim_thread sim_terminal st2_src lc2_src mem2_src e2_tgt.(Thread.state) e2_tgt.(Thread.local) e2_tgt.(Thread.memory)>>.
+    <<SIM: sim_thread sim_terminal st2_src lc2_src sc2_src mem2_src e2_tgt.(Thread.state) e2_tgt.(Thread.local) e2_tgt.(Thread.sc) e2_tgt.(Thread.memory)>>.
 Proof.
-  revert st1_src lc1_src mem1_src MEMORY WF_SRC WF_TGT MEM_SRC MEM_TGT SIM.
+  revert MEMORY WF_SRC WF_TGT SC_SRC SC_TGT MEM_SRC MEM_TGT SIM.
+  revert st1_src lc1_src sc1_src mem1_src.
   induction STEPS; i.
-  { eexists _, _, _. splits; eauto. }
+  { eexists _, _, _, _. splits; eauto. }
   inv H. destruct x, y. ss.
   exploit sim_step; eauto. i. des.
   exploit IHSTEPS; eauto. i. des.
   destruct z. ss.
-  eexists _, _, _. splits; try apply MEMORY1; eauto.
+  eexists _, _, _, _. splits; try apply MEMORY1; eauto.
   etrans; [eauto|]. econs 2; eauto. econs; eauto. etrans; eauto.
 Qed.
 
 Lemma sim_thread_consistent
       lang_src lang_tgt
       sim_terminal
-      st_src lc_src mem_src
-      st_tgt lc_tgt mem_tgt
-      (SIM: sim_thread sim_terminal st_src lc_src mem_src st_tgt lc_tgt mem_tgt)
+      st_src lc_src sc_src mem_src
+      st_tgt lc_tgt sc_tgt mem_tgt
+      (SIM: sim_thread sim_terminal st_src lc_src sc_src mem_src st_tgt lc_tgt sc_tgt mem_tgt)
       (MEMORY: Memory.sim mem_tgt mem_src)
       (WF_SRC: Local.wf lc_src mem_src)
       (WF_TGT: Local.wf lc_tgt mem_tgt)
+      (SC_SRC: Memory.closed_timemap sc_src mem_src)
+      (SC_TGT: Memory.closed_timemap sc_tgt mem_tgt)
       (MEM_SRC: Memory.closed mem_src)
       (MEM_TGT: Memory.closed mem_tgt)
-      (CONSISTENT: Thread.consistent (Thread.mk lang_tgt st_tgt lc_tgt mem_tgt)):
-  Thread.consistent (Thread.mk lang_src st_src lc_src mem_src).
+      (CONSISTENT: Thread.consistent (Thread.mk lang_tgt st_tgt lc_tgt sc_tgt mem_tgt)):
+  Thread.consistent (Thread.mk lang_src st_src lc_src sc_src mem_src).
 Proof.
   generalize SIM. intro X.
   punfold X. exploit X; eauto; try refl. i. des.
@@ -354,7 +375,7 @@ Proof.
   i. des. destruct e2. ss.
   punfold SIM0. exploit SIM0; eauto; try refl. i. des.
   exploit PROMISES1; eauto. i. des.
-  eexists (Thread.mk _ _ _ _). splits; [|eauto].
+  eexists (Thread.mk _ _ _ _ _). splits; [|eauto].
   etrans; eauto.
 Qed.
 
@@ -362,24 +383,24 @@ Qed.
 Lemma sim_thread_sim
       lang_src lang_tgt
       sim_terminal
-      st1_src lc1_src mem_k_src
-      st1_tgt lc1_tgt mem_k_tgt
+      st1_src lc1_src sc_k_src mem_k_src
+      st1_tgt lc1_tgt sc_k_tgt mem_k_tgt
       tid
       (SIM: @sim_thread lang_src lang_tgt sim_terminal
-                        st1_src lc1_src mem_k_src
-                        st1_tgt lc1_tgt mem_k_tgt):
+                        st1_src lc1_src sc_k_src mem_k_src
+                        st1_tgt lc1_tgt sc_k_tgt mem_k_tgt):
   sim
-    (IdentMap.singleton tid (existT _ _ st1_src, lc1_src)) mem_k_src
-    (IdentMap.singleton tid (existT _ _ st1_tgt, lc1_tgt)) mem_k_tgt.
+    (IdentMap.singleton tid (existT _ _ st1_src, lc1_src)) sc_k_src mem_k_src
+    (IdentMap.singleton tid (existT _ _ st1_tgt, lc1_tgt)) sc_k_tgt mem_k_tgt.
 Proof.
-  revert st1_src lc1_src mem_k_src st1_tgt lc1_tgt mem_k_tgt SIM. pcofix CIH. i. pfold. ii.
+  revert st1_src lc1_src sc_k_src mem_k_src st1_tgt lc1_tgt sc_k_tgt mem_k_tgt SIM. pcofix CIH. i. pfold. ii.
   exploit singleton_consistent_inv; try apply WF_SRC; eauto. i. des.
   exploit singleton_consistent_inv; try apply WF_TGT; eauto. i. des.
   splits.
   - i. apply (singleton_is_terminal tid) in TERMINAL_TGT. des.
     punfold SIM0. exploit SIM0; eauto. i. des.
     exploit TERMINAL; eauto. i. des.
-    eexists _, _. splits; [|eauto|].
+    eexists _, _, _. splits; [|eauto|].
     + generalize (rtc_tail STEPS). intro X. des. inv X0.
       * destruct a2. econs 2; [|econs 1].
         econs. rewrite <- TAU. econs; ss; eauto.
@@ -401,7 +422,7 @@ Proof.
     { eapply sim_thread_future; eauto. }
     i. des. destruct e2. ss.
     exploit sim_step; try apply MEMORY; eauto. i. des.
-    eexists _, _, _, _, _, _. splits; eauto.
+    eexists _, _, _, _, _, _, _, _. splits; eauto.
     + econs; s.
       * apply IdentMap.singleton_eq.
       * etrans; eauto.
